locations.v

src/indexing.v
@@ -15,22 +15,25 @@ Definition plend (pl: PathLoc) := match pl with (_, l) => l end.
 
 Section Indexing.
 
-Context {M: Type}  `{!EqDecision M, !Countable M}.
+(*Context {M: Type}  `{!EqDecision M, !Countable M}.*)
 (*Context `{!EqDecision RefinementIndex}.
 Context {refinement_of_index : RefinementIndex -> Refinement M M}.*)
 
-Definition node_of_pl (branch: Branch M) (pl: PathLoc) : Node M. Admitted.
-Definition cell_of_pl (branch: Branch M) (pl: PathLoc) : Cell M. Admitted.
-Definition every_node (branch: Branch M) (fn : Node M -> nat -> Prop) : Prop. Admitted.
+Definition node_of_pl {M} `{!EqDecision M, !Countable M, !TPCM M}
+    (branch: Branch M) (pl: PathLoc) : Node M. Admitted.
+    
+Definition cell_of_pl {M} `{!EqDecision M, !Countable M, !TPCM M}
+    (branch: Branch M) (pl: PathLoc) : Cell M. Admitted.
+    
+Definition every_node {M} `{!EqDecision M, !Countable M, !TPCM M}
+    (branch: Branch M) (fn : Node M -> nat -> Prop) : Prop. Admitted.
 
-Context `{!TPCM M}.
-
-Lemma every_node_equiv_forall
+Lemma every_node_equiv_forall {M} `{!EqDecision M, !Countable M, !TPCM M}
     (branch : Branch M) (fn : Node M -> nat -> Prop)
     (rtriv: ∀ n idx , node_trivial n -> fn n idx)
   : (every_node branch fn) <-> (forall pl , fn (node_of_pl branch pl) (plend pl)). Admitted.
 
-Lemma forall_node_op
+Lemma forall_node_op {M} `{!EqDecision M, !Countable M, !TPCM M}
     (branch1 : Branch M) (branch2 : Branch M)
   : forall pl , (node_of_pl branch1 pl) ⋅ (node_of_pl branch2 pl) ≡ node_of_pl (branch1 ⋅ branch2) pl.
 Admitted.
