src/locations.v
@@ -1,0 +1,74 @@
+From iris.algebra Require Export cmra.
+From iris.algebra Require Import proofmode_classes.
+From iris.prelude Require Import options.
+Require Import Burrow.CpdtTactics.
+
+From stdpp Require Import gmap.
+From stdpp Require Import mapset.
+From stdpp Require Import sets.
+From stdpp Require Import list.
+Require Import Burrow.gmap_utils.
+Require Import Burrow.rollup.
+Require Import Burrow.indexing.
+
+(*Context {M: Type} `{!EqDecision M, !TPCM M} `{!Countable M}.
+Context `{Countable RefinementIndex}.
+Context `{EqDecision RefinementIndex}.
+Context (ref_map : RefinementIndex -> Refinement M M).*)
+
+Inductive Loc (RI: Type) `{!EqDecision RI, !Countable RI} :=
+  | BaseLoc : nat -> Loc RI
+  | ExtLoc : nat -> RI -> Loc RI -> Loc RI
+  | CrossLoc : Loc RI -> Loc RI -> Loc RI
+.
+
+Definition pls_of_loc `{Countable RI} (loc: Loc RI) : (listset PathLoc). Admitted.
+
+Definition build `{Countable RI} {M} `{!EqDecision M, !Countable M, !TPCM M}
+    (loc: Loc RI) (cell: Cell M) : Branch M. Admitted.
+    
+Lemma build_spec `{Countable RI} {M} `{!EqDecision M, !Countable M, !TPCM M}
+    (loc: Loc RI) (cell: Cell M)
+  : (∀ pl , pl ∈ pls_of_loc loc -> cell_of_pl (build loc cell) pl = cell). Admitted.
+  
+Lemma build_rest_triv
+        {M} `{!EqDecision M, !Countable M, !TPCM M}
+        {RI} `{!EqDecision RI, !Countable RI}
+    (loc: Loc RI) (cell: Cell M)
+  : (∀ pl , ¬(pl ∈ pls_of_loc loc) -> cell_trivial (cell_of_pl (build loc cell) pl)). Admitted.
+
+Definition refinement_of_index
+        M `{!EqDecision M, !Countable M, !TPCM M}
+        RI `{!EqDecision RI, !Countable RI}
+        (idx: nat) : Refinement M M. Admitted.
+
+(*
+Global Instance loc_eqdec : EqDecision Loc.
+Proof. solve_decision. Defined.
+
+Global Instance loc_countable : Countable Loc.
+Proof.
+  set (enc :=
+    fix go l :=
+      match l with
+      | BaseLoc i => GenLeaf (inl i)
+      | ExtLoc i ri linner => GenNode 0 [GenLeaf (inr (i, ri)); go linner]
+      | CrossLoc l1 l2 => GenNode 1 [go l1; go l2]
+      end
+  ).
+  set (dec :=
+    fix go e :=
+      match e with
+      | GenLeaf (inl i) => BaseLoc i
+      | GenNode 0 [GenLeaf (inr (i, ri)); einner] => ExtLoc i ri (go einner)
+      | GenNode 1 [e1; e2] => CrossLoc (go e1) (go e2)
+      | _ => BaseLoc 0 (* dummy *)
+      end
+  ).
+  refine (inj_countable' enc dec _).
+  refine (fix go (e : Loc) {struct e} := _).
+  - destruct e as [| | ]; simpl; f_equal; trivial.
+Qed.
+
+Inductive ILoc
+*)
